merge from demo branch

core/Prog.v
@@ -1,4 +1,4 @@
-Require Import Monads List ZArith Program.
+Require Import Monads ProofMonads List ZArith Program.
 
 Open Scope monad_scope.
 
@@ -6,145 +6,126 @@ Import ListNotations.
 
 Set Implicit Arguments.
 
+Module M := Monads.
+Module PM := ProofMonads.
+
 Section Test.
 
 Definition init_val1 := 0.
 
 Definition init_S1 : nat := init_val1.
 
-Print modify.
+Definition add_s (i : nat) : M.State nat unit :=
+  M.modify (fun s => s + i).
 
-Definition add_s (i : nat) : Monads.State nat unit :=
-  Monads.modify (fun s => s + i).
-
-Definition minus_s (i : nat) : Monads.State nat unit :=
-  Monads.modify (fun s => s - i).
+Definition minus_s (i : nat) : M.State nat unit :=
+  M.modify (fun s => s - i).
 
 Definition get10 : State nat nat:= return_ 10.
 
-Definition count15 : State nat unit :=
- add_s 1;;
- add_s 2;;
- add_s 3;;
- add_s 4;;
- add_s 5;;
- return_ tt.
-
-Notation "{{ P }} m {{ Q }}" := (hoareTripleS P m Q)
-  (at level 90, format "'[' '[' {{  P  }}  ']' '/  ' '[' m ']' '['  {{  Q  }} ']' ']'") : monad_scope.
-
-Lemma l_add_s :
- forall (n i : nat), {{fun (s : nat) => s = n}} add_s i {{fun (_ : unit) (s : nat) => s = n + i}}.
-  Proof.
-  intros n i s H.
-  unfold add_s.
-  apply l_modify.
-  auto.
-  Qed.
-
-Lemma l_count15 : {{fun s : nat => s = init_S1}} count15 {{fun (_ : unit ) (s : nat) => s = 15}}.
-  Proof.
-  apply bindRev with (Q := (fun (_ : unit ) (s : nat) => s = 1)); try apply l_add_s.
-  + intros; apply bindRev with (Q := (fun (_ : unit ) (s : nat) => s = 3)) ; try apply l_add_s.
-  - intros; apply bindRev with (Q := (fun (_ : unit ) (s : nat) => s = 6)) ; try apply l_add_s.
-  * intros; apply bindRev with (Q := (fun (_ : unit ) (s : nat) => s = 10)) ; try apply l_add_s.
-    intros; apply bindRev with (Q := (fun (_ : unit ) (s : nat) => s = 15)) ; try apply l_add_s.
-    intros. intros S H. trivial.
-  Qed.
-
-Definition count42 : State nat unit
- := for j = 0 to 3 {{ 
-    add_s j ;;
-    add_s j ;;
-    perf x <- get10;
-    add_s x ;;
-    add_s j ;;
-    add_s j
-  }} .
-
-Definition counti : State nat () :=
-   for i = 0 to 20 {{
-    (add_s i)
-  }}.
-
-Lemma l_counti : hoareTripleS (fun s : nat => s = init_S1) counti (fun (_ : unit ) (s : nat) => s = 42).
-  Proof.
-  eapply bindRev.
-  Admitted.
-
-Lemma l_count42 : hoareTripleS (fun s : nat => s = init_S1) count42 (fun (_ : unit ) (s : nat) => s = 42).
-  Proof.
-  eapply bindRev.
-  unfold count42.
-  unfold loopT_liftT.
-  eapply bindRev.
-  Admitted.
-
-Check count42.
+Compute runState (
+  for i = 5 to 0 {{
+    add_s 1
+  }}) init_S1.
 
 Compute runState (
-  count42
-  ) init_S1.
+  for2 i = 5 to 0 {{
+    add_s 1
+  }}) init_S1.
 
 Compute runState (
-  for i = 0 to 5 {{
+  for i = 5 to 0 {{
+    add_s i 
+  }}) init_S1.
+(* 4 + 3 + 2 + 1 + 0 = 10 *)
+
+Compute runState (
+  for2 i = 5 to 0 {{
+    add_s i 
+  }}) init_S1.
+
+Compute runState (
+  for i = 5 to 0 {{
     add_s i 
   }} ;; 
-  for j = 0 to 5 
+  for j = 5 to 0 
   {{ 
     add_s j 
   }} ) init_S1.
 
 Compute runState (
-  for i = 0 to 5 {{
+  for2 i = 5 to 0 {{
+    add_s i 
+  }} ;; 
+  for2 j = 5 to 0 
+  {{ 
+    add_s j 
+  }} ) init_S1.
+
+Compute runState (
+  for i = 5 to 0 {{
     add_s i 
   }} ;; 
   perf x <- get10 ;
   add_s x ;;
-  for j = 0 to 5 
+  for j = 5 to 0 
+  {{ 
+    add_s j 
+  }} ) init_S1.
+  
+Compute runState (
+  for2 i = 5 to 0 {{
+    add_s i 
+  }} ;; 
+  perf x <- get10 ;
+  add_s x ;;
+  for2 j = 5 to 0 
   {{ 
     add_s j 
   }} ) init_S1.
 
-Open Scope list_scope.
+Compute runState (
+   for_e i = 20 to 0 {{
+    if (i =? 15) then exit
+    else (loopT_liftT (add_s i))
+  }} ) init_S1.
+(* 19 + 18 + 17 + 16 = 70 *)
 
-Definition nth2 := 4.
+Open Scope list_scope.
 
 Definition init_S2 : list nat := [].
 
 Definition addElement (val : nat) : State (list nat) unit :=
-  modify (fun s => val :: s).
+  M.modify (fun s => val :: s).
 
-Compute runState (for i = 0 to nth2 {{ for j = 0 to nth2 {{addElement (i+j) }} }} ) init_S2.
+Compute runState (
+  for i = 5 to 0 {{
+    for j = 3 to 0 {{
+      addElement (i + j) 
+    }} 
+  }}) init_S2.
 
-(* exit *)
-
-Definition test_exit : State nat () :=
-   for_e i = 0 to 20 {{
-    if (i =? 5) then exit
-    else (loopT_liftT (add_s i))
-  }}.
-
-
-Lemma l_test_exit : hoareTripleS (fun s : nat => s = 0) test_exit (fun (_ : unit ) (s : nat) => s = 0).
-  Proof.
-  eapply bindRev.
-  Admitted.
+Compute runState (
+  for2 i = 5 to 0 {{
+    for2 j = 3 to 0 {{
+      addElement (i + j) 
+    }} 
+  }}) init_S2.
 
 Open Scope Z_scope.
 
 (* if/else *)
 
-Definition add_z (i : nat) : Monads.State Z unit :=
-  Monads.modify (fun s => s + Z.of_nat i).
+Definition add_z (i : nat) : M.State Z unit :=
+  M.modify (fun s => s + Z.of_nat i).
 
-Definition minus_z (i : nat) : Monads.State Z unit :=
-  Monads.modify (fun s => s - Z.of_nat i).
+Definition minus_z (i : nat) : M.State Z unit :=
+  M.modify (fun s => s - Z.of_nat i).
 
 Definition init_Z1 : Z := 0.
 
 Compute runState (
-  for i = 0 to 6 {{
+  for i = 6 to 0 {{
     if (Z.eqb (Z.modulo (Z.of_nat i) 2) 0) then
       add_z i 
     else 
